RAC of arithmetic properties: lemma C.1

Definitions.v
@@ -5,167 +5,235 @@ From Coq Require Import Strings.String.
 Open Scope Z_scope.
 Open Scope fsl_scope.
 
-Inductive p_type := PInt | Void.
-Inductive l_type := LInt | Integer.
 
-Inductive c_binop_int := Add | Min | Mul | Div.
-Inductive c_binop_bool :=  Lt | Le | Gt | Ge | Eq | NEq.
+Inductive c_type := C_Int | Void.  (* program types τc *)
+Inductive gmp_t := Ctype (t:c_type) | String | Mpz. (* type extension τ *)
 
-Inductive fsl_binop_bool :=  FSLLt | FSLLe | FSLGt | FSLGe | FSLEq | FSLNEq.
-Inductive fsl_binop_int := FSLAdd | FSLMin  | FSLMul  | FSLDiv.
+(* mini-FSL *)
+
+Inductive fsl_decl :=  FSL_Decl (τ:gmp_t) (name:id). (* logic declaration δ *)
+Inductive fsl_binop_bool :=  FSL_Lt | FSL_Le | FSL_Gt | FSL_Ge | FSL_Eq | FSL_NEq.
+Inductive fsl_binop_int := FSL_Add | FSL_Min  | FSL_Mul  | FSL_Div.
+
+Inductive predicate :=
+    | P_True | P_False (* truth values *)
+    | P_BinOp (lt: fsl_term) (op:fsl_binop_bool) (rt : fsl_term)
+    | Not (t:fsl_term)
+    | Disj (lp:predicate) (rp:predicate)  (* disjunction *)
+    | Call (name:string) (args:fsl_decl^*) (* predicate call *)
+with fsl_term :=
+    | T_Z (z:Z) (* integer in Z *)
+    | T_Id (name:id) (* variable access *)
+    | T_BinOp (lt : fsl_term) (op:fsl_binop_int) (rt : fsl_term)
+    | Conditional (cond:predicate) (_then:fsl_term) (_else:fsl_term) (* conditional term *)
+.
 
 
+Inductive fsl_type := FSL_Int | Integer. (* logic types *)
+   
+
+(* mini-C *)
+Inductive c_decl :=  C_Decl (type:c_type) (name:id). (* program declaration *)
+
+Inductive c_binop_bool :=  C_Lt | C_Le | C_Gt | C_Ge | C_Eq | C_NEq.
 Definition c_binop_bool_model (x:c_binop_bool) : Z -> Z -> Prop := match x with
-    | Lt => Z.lt
-    | Le => Z.le
-    | Gt => Z.gt
-    | Ge => Z.ge
-    | Eq => Z.eq
-    | NEq => fun b1 b2 => ~ (Z.eq b1 b2)
+    | C_Lt => Z.lt
+    | C_Le => Z.le
+    | C_Gt => Z.gt
+    | C_Ge => Z.ge
+    | C_Eq => Z.eq
+    | C_NEq => fun b1 b2 => ~ (Z.eq b1 b2)
 end.
 Notation "◁" := c_binop_bool_model.
 
+Inductive c_binop_int := C_Add | C_Min | C_Mul | C_Div. 
 Definition c_binop_int_model (x:c_binop_int) : Z -> Z -> Z := match x with
-    | Add => Z.add
-    | Min => Z.min
-    | Mul => Z.mul
-    | Div => Z.div
+    | C_Add => Z.add
+    | C_Min => Z.min
+    | C_Mul => Z.mul
+    | C_Div => Z.div
 end.
 Notation "⋄" := c_binop_int_model.
 
-Notation id := string.
 
-Inductive mini_c_exp :=
-    | Zm (z : Z)
-    | Id (id : string)
-    | BinOpInt (exp : mini_c_exp) (op:c_binop_int) (exp : mini_c_exp)
-    | BinOpBool (exp : mini_c_exp) (op:c_binop_bool) (exp : mini_c_exp)
+Inductive c_exp :=
+    | Zm (z : Z) (* machine integer *)
+    | C_Id (var : id) (* variable access *)
+    | BinOpInt (le : c_exp) (op:c_binop_int) (re : c_exp)
+    | BinOpBool (le : c_exp) (op:c_binop_bool) (re : c_exp)
     .
 
-     Inductive mini_fsl.
-     
-     Inductive c_statement :=
-         | Skip
-         | Assign (vname:id) (exp: mini_c_exp)
-         | FCall (var:id) (fname:id) (args: list mini_c_exp)
-         | PCall  (pname:id) (args: list mini_c_exp)
-         | Seq (s1 : c_statement) (s2 : c_statement)
-         | If (cond:mini_c_exp) (_then:c_statement) (_else:c_statement)
-         | While (cond:mini_c_exp) (body:c_statement)
-         | PAssert (e:mini_c_exp)
-         | LAssert (a:mini_fsl)
-         | Return (e:mini_c_exp)
-         .
-     
-     
-     (* begin mini-GMP *)
-     Inductive t_ext := Ptype (t:p_type) | String | tMpz.
-     
-     Inductive g_statement := 
-         | Init (id:id)
-         | Set_i (id:id) (e:mini_c_exp)
-         | Set_s (id:id) (l:string)
-         | Set_z (lid rid:id)
-         | Clear (id:id)
-         | GAdd (lid rid res :id)
-         | GSub (lid rid res :id)
-         | GMul (lid rid res :id)
-         | GDiv (lid rid res :id)
-         | Comp (res lid rid :id) 
-         | Coerc (res n : id)
-         .
-     
-     Inductive statement := SMpz (s:g_statement) | SCommand (c:c_statement).
-     
-     (* end mini-GMP *)
-     
-     
-     
-     Inductive p_decl :=  PDecl (ty:p_type) (id:id).
-     Inductive l_decl :=  LDecl (ty:t_ext) (id:id).
-     
-     
-     Inductive predicate :=
-         | FSLTrue
-         | FSLFalse
-         | Not (t:mini_fsl_term)
-         | Disj (p1:predicate) (p2:predicate)
-         | FSLPCall (name:id) (args:list l_decl)
-         | FSLBinOpBool (t1: mini_fsl_term) (op:fsl_binop_bool) (t2 : mini_fsl_term)
-     
-     with mini_fsl_term :=
-         | FSLZ (n:Z)
-         | FSLId (id:string)
-         | FSLBinOpInt (t1 : mini_fsl_term) (op:fsl_binop_int) (t2 : mini_fsl_term)
-         | Conditional (cond:predicate) (_then:mini_fsl_term) (_else:mini_fsl_term)
-         .
-     
-     
-     Inductive mini_c_routines :=
-         | PFun (rt:p_type) (name:id) (args: list p_decl) (decl: list p_decl ) (body:statement)
-         | LFun (rt:l_type) (name:id) (args:list l_decl)
-         | Predicate (name:id) (p:mini_fsl_term)
-         .
-     
-     Inductive mini_c := Program (decls: list p_decl)  (routines: list mini_c_routines).
-     
+Inductive c_statement :=
+| Skip (* empty statement *)
+| Assign (var:id) (e: c_exp) (* assignment *)
+| FCall (var:string) (fname:string) (args: c_exp^*) (* function call *)
+| PCall  (fname:string) (args: c_exp^*) (* procedure call *)
+| Seq (s1 : c_statement) (s2 : c_statement) (* sequence *)
+| If (cond:c_exp) (_then:c_statement) (_else:c_statement) (* conditional *)
+| While (cond:c_exp) (body:c_statement) (* loop *)
+| PAssert (e:c_exp) (* program assertion *)
+| LAssert (p:predicate) (* logic assertion *)
+| Return (e:c_exp)
+.
 
-Definition V : Set := id. (* program variables *)
+Inductive c_routines :=
+| PFun (ret:c_type) (name:id) (args: c_decl^*) (b_decl: c_decl^* ) (body:c_statement) (* program function *)
+| LFun (ret:fsl_type) (name:id) (args: fsl_decl^*) (body:fsl_term) (* logic function *)
+| Predicate (name:id) (args: fsl_decl^*) (p:predicate) (* predicate *)
+.
+
+Inductive c_program := Program (decls: c_decl^*)  (routines: c_routines^*).  (* annotated program *)
+
+     
+(*  mini-GMP *)
+
+Inductive gmp_statement := 
+    | Init (name:id) (* mpz allocation *)
+    | Set_i (name:id) (e:c_exp) (* assignment from an int *)
+    | Set_s (name:id) (l:string) (* assignment from a string literal *)
+    | Set_z (name z:id)(* assignment from a mpz *)
+    | Clear (name:id) (* mpz de-allocation *)
+    | GMP_Add (lid rid res :id)
+    | GMP_Sub (lid rid res :id)
+    | GMP_Mul (lid rid res :id)
+    | GMP_Div (lid rid res :id)
+    | Comp (res lid rid :id) (* mpz comparison *)
+    | Coerc (name n : id) (* mpz coercion *)
+    .
+
+Inductive statement := S_G (s:gmp_statement) | S_C (c:c_statement). (* statement extension *)
+   
+     
+Definition V : Set := id. (* program variables and routines *)
 
 #[global] Instance eqdec_v : EqDec V := {eq_dec := string_dec}.
 
 Definition S : Set := c_statement. (* program statements *)
-Definition L : Set := l_decl. (* logic variables *)
-Definition Z : Set := mini_fsl_term. (* logical terms *)
+Definition L : Set := fsl_decl. (* logic variables and routines *)
+Definition LT : Set := fsl_term. (* logical terms *)
 Definition B : Set := predicate. (* predicates *)
-Definition T : Set := t_ext. (* minigmp types *)
+Definition T : Set := gmp_t. (* minigmp types *)
 
-Definition F : V ⇀ (V^* -> S). Admitted. (* program functions *)
-Definition P : V ⇀ (V^* -> S). Admitted. (* program procedures *)
-Definition Fl :  L ⇀ (L^* -> Z). Admitted. (* logic functions *)
-Definition Bl :  L ⇀ (L^* -> B). Admitted. (* predicates *)
+(* ty the function that gives the type of a mini-GMP expression  -> where are the expressions defined ? *)
 
-
-(*
-
-m_int M_int : lower and upper bounds of type int 
-*)
-
-Definition m_int : BinNums.Z := -10.
-Definition M_int : BinNums.Z := 10.
+Definition F := V ⇀ (V^* -> S). (* program functions *)
+Definition P := V ⇀ (V^* -> S). (* program procedures *)
+Definition Fl :=  L ⇀ (L^* -> Z). (* logic functions *)
+Definition Bl :=  L ⇀ (L^* -> B). (* predicates *)
 
 
-Definition Int : Set := Z. (* set of type int, a machine integer (may overflow) *)
+Module Int16Bounds.
+    Definition m_int := -32768.
+    Definition M_int := 32767.
+End Int16Bounds.
+
+Module Int := MachineInteger Int16Bounds.
+
+Lemma zeroinRange : Int.inRange 0.
+Proof.
+    split ; reflexivity.
+Qed.
+
+Lemma oneinRange : Int.inRange 1.
+Proof.
+    split ; reflexivity.
+Qed.
+
+Inductive Values := 
+    | Int (n:Int.MI) (* set of type int, a machine integer (may overflow) *)
+    | VMpz (n:nat)  (* memory location for values of type mpz *) 
+    | UInt   (* set of undefined values of type int *) 
+    | UMpz  . (* set of undefined values of type mpz *) 
+
+Definition values_int (v:Values) : option Values := match v with
+| Int n => Some (Int n)
+| _ => None
+end.
 
 
-Definition Mpz  : Set :=  Empty_set.  (* memory location for value of type mpz *) 
-
-Definition Uint  : Set := Empty_set. (* set of undefined values of type int *) 
-Definition Umpz  : Set :=  Empty_set.  (* set of undefined values of type mpz *) 
-
-(* Infix  "⊎" := Sets.Ensembles.Union (at level 10). *) 
-
-(*set of values an expression may evaluate to *)
-(* Definition Values : (Int * Mpz * Uint * Umpz)%type. *)
-
-(* Inductive Values : Set := Int (n:Z) | Mpz (n:option Z) | Uint | Umpz.  *)
-
-Inductive Values := VInt (n:Int) | VMpz (n:Mpz) | VUint (n:Uint) | VUMpz (n:Umpz) .
-
-(*
 (* integer from value *)
-Definition z_of_Int : Int -> Z := fun x => match x with Int => 0 end.
-*)
+Definition z_of_Int : Int.MI -> Z := Int.to_z.
 
-Definition M := Mpz ⇀ Z. (* memory state, i.e. current mpz value of given mem loc*)
-
+Definition M := nat ⇀ Z. (* memory state, i.e. current mpz value of given mem loc*)
 
 Definition Ωᵥ := V ⇀ Values.
-Definition Ωₗ := L ⇀ Values.
+Definition Ωₗ := L ⇀ Z.
 
-Definition Ω := (Ωᵥ * Ωₗ)%type. (* semantic env *)
+(* Record Ω := {decl_env: Ωᵥ; logic_env: Ωₗ}. (* semantic env *) *)
 
-Definition Γ  := mini_c_routines -> T. (* typing env *)
+Definition Ω := (Ωᵥ * Ωₗ)%type.
+
+Definition Γ  := c_routines -> T. (* typing env *)
+
+Record I := {min : Z; max : Z}. (* interval *)
+
+
+Definition Γᵢ := L ⇀ I. (* typing env mapping logic binders to  intervals *)
+
+
+Definition oracle := LT -> Γᵢ -> I.
+
+Definition Θ :=  I -> T.
+
+Definition Tr (o: oracle) (om:Θ) : LT -> Γᵢ -> T := fun lt env => om (o lt env). (* Θ ◦ oracle. *)
+
+
+
+Coercion C_Id : string >-> c_exp.
+Coercion Zm : Z >-> c_exp.
+(* Coercion Int.of_z : Z >-> Int.MI. *)
+Coercion Int : Int.MI >-> Values. 
+Coercion VMpz : nat >-> Values.
+
+
+
+Definition same_values (v1 v2: option Values) : bool := match v1,v2 with
+    | Some (Int n1), Some (Int n2) =>  Int.mi_eq n1 n2
+    | Some (VMpz n1), Some (VMpz n2) => (n1 =? n2)%nat
+    | _,_ => false
+end
+.
+
+
+Definition env_partial_orderb (env:Ω) (env':Ω) (v:V) : bool :=
+    let venv := fst env in
+    let venv' := fst env' in 
+     match venv v with 
+        | Some (Int _) | Some (VMpz _) => same_values (venv v) (venv' v)
+        | Some UInt => match venv' v with 
+            | Some UInt | Some (Int _) => true
+            | _ => false
+            end
+        | Some UMpz => match venv' v with 
+            | Some UMpz | Some (VMpz _) => true
+            | _ => false
+            end
+        | None => true
+    end
+.
+
+Inductive env_partial_order (env:Ω) (env':Ω) (v:id) : Prop :=
+| sameInt n: 
+    (fst env) v = Some (Int n)
+    -> (fst env') v = Some (Int n)
+    -> env_partial_order env env' v
+| sameMpz n: 
+    (fst env) v = Some (VMpz n)
+    -> (fst env') v = Some (VMpz n)
+    -> env_partial_order env env' v
+| undefInt n : (fst env) v = Some UInt
+    -> (fst env') v = Some UInt \/ (fst env') v = Some (Int n)
+    -> env_partial_order env env' v
+| undefMpz n : (fst env) v = Some UMpz
+    -> (fst env') v = Some UMpz \/ (fst env') v = Some (VMpz n)
+    -> env_partial_order env env' v
+| none : (fst env) v = None -> env_partial_order env env' v
+.
+
+
+
+Notation "e ⊑ e'" := (forall v, env_partial_order e e' v) (at level 99).
+
 
 
 (* Module Todo.
