Utils.v
@@ -1,5 +1,7 @@
 From RAC Require Import Notations.
 From Coq Require Import ZArith.ZArith.
+From Coq Require Import Setoids.Setoid.
+
 Open Scope Z_scope.
 
 
@@ -18,7 +20,7 @@ Class EqDec X :=
 Definition p_map {X Y : Type} `{EqDec X}  (f: X -> option Y) (x:X) (y:Y) : X -> option Y :=
     fun i => if eq_dec x i then Some y else f i.
 
-Notation "f { x \ y }" := (p_map f x y) : fsl_scope.
+Notation "f { x \ y }" := (p_map f x y): fsl_scope.
 
 
 Inductive domain { X Y : Type} (f: X ⇀ Y) (y:Y) := 
@@ -28,16 +30,80 @@ Inductive domain { X Y : Type} (f: X ⇀ Y) (y:Y) :=
 Notation "'dom' f" := (domain f) : fsl_scope.
 
 
+Module Type Bounds.
+    Parameter m_int : Z.
+    Parameter M_int : Z.
+End Bounds.
 
-(*
+(* simplified from compcert.lib.Integers *)
+Module MachineInteger(B:Bounds).
+    Definition inRange n :=B.m_int < n < B.M_int.
 
- Inductive p_map {X Y : Type} (f: X ⇀ Y) (x:X) (y:Y) : X -> option Y -> Prop := 
-    | is_x : f { x \ y } x (Some y)
-    | is_not_x : 
-        forall (i:X), i <> x -> 
-        forall (o: option Y), (f i) = o -> 
-        f { x \ y } i o
+    Record MI := mkMI {val : Z; in_range : inRange val}.
+    
+    Definition to_z (i:MI) : Z := i.(val).
+    Definition of_z (val:Z) H : MI := mkMI val H.
+    Definition mi_eq m1 m2 := val m1 =? val m2.
+    Axiom eq : forall m1 m2, val m1 = val m2 <-> m1 = m2.
 
- where "f { x \ y }" := (p_map f x y). 
- *)
+    Lemma mi_eq_iff : forall m1 m2, mi_eq m1 m2 = true <-> m1 = m2.
+    Proof.
+      intros m1 m2. split.
+      - intros H. unfold mi_eq in H. apply Z.eqb_eq in H. apply eq in H. apply H.
+      - intro H. rewrite H. apply Z.eqb_refl.
+    Qed.
+   (* Definition eq m1 m2 := Z.eq_dec (val m1)  (val m2).
+
+
+   Lemma mkint_eq:
+   forall x y Px Py, x = y -> mkMI x Px = mkMI y Py.
+ Proof.
+   intros. subst y.
+   assert (forall (n m: Z) (P1 P2: n < m), P1 = P2).
+   {
+     unfold Z.lt; intros.
+     apply Eqdep_dec.eq_proofs_unicity.
+     intros c1 c2. destruct c1; destruct c2; (left; reflexivity) || (right; congruence).
+   }
+   destruct Px as [Px1 Px2]. destruct Py as [Py1 Py2].
+   rewrite (H _ _ Px1 Py1).
+   rewrite (H _ _ Px2 Py2).
+   reflexivity.
+ Qed.
+
+   Lemma eq_dec: forall (x y: MI), {x = y} + {x <> y}.
+    Proof.
+    intros. destruct x; destruct y. destruct (Z.eq_dec val0 val1).
+    left. apply mkint_eq. auto.
+    right. red; intro. injection H. exact n.
+    Qed.
+
+    Lemma zeq_true:
+    forall (A: Type) (x: Z) (a b: A), (if Z.eq_dec x x then a else b) = a.
+  Proof.
+    intros. case (Z.eq_dec x x); intros.
+    auto.
+    elim n; auto.
+  Qed.
+
+  Lemma zeq_false:
+  forall (A: Type) (x y: Z) (a b: A), x <> y -> (if Z.eq_dec x y then a else b) = b.
+Proof.
+  intros. case (Z.eq_dec x y); intros.
+  auto.
+  elim H; auto. auto.
+Qed.
+
+
+Theorem eq_spec: forall (m1 m2: MI), if eq m1 m2 then m1 = m2 else m1 <> m2.
+Proof.
+    intros; unfold eq. case (eq_dec m1 m2); intro.
+    subst m2. rewrite zeq_true. auto.
+    rewrite zeq_false. auto.
+    destruct m1; destruct m2.
+    simpl. red; intro. elim n. apply mkint_eq. auto.
+Qed. *)
+
+End MachineInteger.
+
 
