Notations.v
@@ -15,13 +15,18 @@ Reserved Notation "⊥".
 Reserved Notation "f { x \ y }" (at level 10).
 Reserved Notation "'dom' f" (at level 10).
 
+Notation id := string.
+
 
 (* Declare Custom Entry exp.
 Declare Custom Entry term.
 Delimit Scope exp_scope with exp. *)
 
-Reserved Notation "Ω '⊨' e => v" (at level 20). (* semantic of expressions, v ∈ Values *)
-(* Reserved Notation "Ω '⊨' t '=>' z" (at level 200).  semantic of terms z ∈ Z*)
-(* Reserved Notation "Ω '⊨' p '=>' b" (at level 200).  semantic of predicates b ∈ Bools *)
+Reserved Notation "Ω ⊨ e => v" (at level 90). (* semantic of expressions, v ∈ Values *)
+(* Reserved Notation "Ω ⊨ t => z" (at level 200).  semantic of terms z ∈ Z*)
+(* Reserved Notation "Ω ⊨ p => b" (at level 200).  semantic of predicates b ∈ Bools *)
 
-Reserved Notation "Ω ',' M '⊨' s '=>' Ω' ',' M'" (at level 200).  (* semantic of statements *)
+(* Reserved Notation "Ω , M ⊨ s => Ω' , M'" (at level 200).  (* semantic of statements *) *)
+
+
+Reserved Notation "e ⊑ e'" (at level 99).
