Semantics.v
@@ -2,72 +2,72 @@ Require Import RAC.Definitions.
 Require Import RAC.Notations.
 Require Import RAC.Utils.
 Require Import ZArith.ZArith.
+From Coq Require Import Strings.String.
 Open Scope fsl_scope.
 Open Scope Z_scope.
 
 
-Inductive mini_c_exp_sem : mini_c_exp -> Ω -> Values ->  Prop :=
-| E_Int z env : env ⊨ (Zm z) => VInt (FSLZ z)
+Inductive c_exp_sem : c_exp -> Ω -> Values -> Prop :=
+| E_Int (z:Z) env in_range: env ⊨ z =>  (Int.of_z z in_range)
 | E_Var (x:V) z (env:Ω) : 
-    (fst env)(x) = Some z -> env ⊨ Id x => z
-| E_BinOpInt env e e' z z' op :
-    env ⊨ e => VInt (FSLZ z) ->
-    env ⊨ e' => VInt (FSLZ z') ->
-    m_int <= (⋄ op) z z' <= M_int ->
-    env ⊨ BinOpInt  (Zm z) op (Zm z) => VInt (FSLZ ((⋄ op) z z'))
-| E_BinOpTrue env e e' z z' op :
-    env ⊨ e => VInt (FSLZ z) ->
-    env ⊨ e' => VInt (FSLZ z') ->
+    (fst env)(x:string) = Some (Int z) -> 
+    env ⊨ x => z
+| E_BinOpInt env e e' (z z':Z) op z_ir z'_ir 
+    (H:Int.inRange (⋄ op z z')) :
+    env ⊨ e =>  (Int.of_z z z_ir) ->
+    env ⊨ e' =>  (Int.of_z z' z'_ir) ->
+    env ⊨ BinOpInt e op e' => Int.of_z ((⋄ op) z z') H
+| E_BinOpTrue env e e' (z z' : Z) z_ir z'_ir op :
+    env ⊨ e => (Int.of_z z z_ir) ->
+    env ⊨ e' => (Int.of_z z z'_ir) ->
     ((◁ op) z z' = True) ->
-    env ⊨ BinOpBool (Zm z) op (Zm z) => VInt (FSLZ 1)
-| E_BinOpFalse env e e' z z' op :
-    env ⊨ e => VInt (FSLZ z) ->
-    env ⊨ e' => VInt (FSLZ z') ->
+    env ⊨ BinOpBool e op e' => Int.of_z 1 oneinRange
+| E_BinOpFalse env e e' (z z' : Z) op z_ir z'_ir :
+    env ⊨ e => (Int.of_z z z_ir) -> 
+    env ⊨ e' => (Int.of_z z' z'_ir) -> 
     ((◁ op) z z' = False) ->
-    env ⊨ BinOpBool (Zm z) op (Zm z) => VInt (FSLZ 0)
+    env ⊨ BinOpBool e op e' => Int.of_z 0 zeroinRange
 
-where  "Ω '⊨' e => v" := (mini_c_exp_sem e Ω v).
+where  "Ω '⊨' e => v" := (c_exp_sem e Ω v).
 
 
-Inductive mini_c_decl_sem : p_decl -> Ω -> p_decl -> Ω -> p_decl -> Prop := 
+Inductive c_decl_sem : c_decl -> Ω -> M -> Ω -> M -> Prop := 
     | Decl (env:Ω) (v := fst env) (l := snd env) mem t x (u:Values) : 
-        v x = ⊥ -> 
-        (* (env,mem ⊨ PDecl t x => (v{x\u},l),mem) *)
-        mini_c_decl_sem (PDecl t x) env mem (v{x\u}, l) mem
+        (* v x = ⊥ -> (env,mem ⊨ C_Decl t x => (v{x\u},l),mem) *)
+        c_decl_sem (C_Decl t x) env mem (v{x\u}, l) mem 
   (* where 
-  "Ω ',' M '⊨' d '=>' Ω' ',' M'" := (mini_c_decl_sem d Ω M Ω' M')  *)
+  "Ω ',' M '⊨' d '=>' Ω' ',' M'" := (c_decl_sem d Ω M Ω' M')  *)
 .
 
 
-Inductive mini_c_stmt_sem : S -> Ω -> M -> Ω -> M -> Prop := 
-    | S_skip env mem : mini_c_stmt_sem Skip env mem env mem
+Inductive c_stmt_sem : S -> Ω -> M -> Ω -> M -> Prop := 
+    | S_skip env mem : c_stmt_sem Skip env mem env mem
     | S_Assign (env:Ω) (v:= fst env) (l:= snd env) mem x z e : 
         (* in v x Int + Uint  *)
         env ⊨ e => z ->
-        mini_c_stmt_sem (Assign x e) env mem (v{x\z},l) mem
+        c_stmt_sem (Assign x e) env mem (v{x\z},l) mem
     | S_IfTrue (env env':Ω) mem mem' z e s s' :
         env ⊨ e => z ->
-        z <> VInt (FSLZ 0) ->
-        mini_c_stmt_sem s env mem env' mem' ->
-        mini_c_stmt_sem (If e s s') env mem env' mem' 
+        z <>  Int.of_z 0 zeroinRange ->
+        c_stmt_sem s env mem env' mem' ->
+        c_stmt_sem (If e s s') env mem env' mem' 
     | S_IfFalse (env env':Ω) mem mem' z e s s' :
         env ⊨ e => z ->
-        z = VInt (FSLZ 0) ->
-        mini_c_stmt_sem s' env mem env' mem' ->
-        mini_c_stmt_sem (If e s s') env mem env' mem' 
+        z = Int.of_z 0 zeroinRange ->
+        c_stmt_sem s' env mem env' mem' ->
+        c_stmt_sem (If e s s') env mem env' mem' 
     | S_While e s env mem env' mem' :
-        mini_c_stmt_sem (If e (Seq s (While e s)) Skip) env mem env' mem' ->
-        mini_c_stmt_sem (While e s) env mem env' mem' 
+        c_stmt_sem (If e (Seq s (While e s)) Skip) env mem env' mem' ->
+        c_stmt_sem (While e s) env mem env' mem' 
     | S_Seq env mem env' mem' env'' mem'' s s' :
-        mini_c_stmt_sem s env mem env' mem' -> 
-        mini_c_stmt_sem s' env' mem' env'' mem'' ->
-        mini_c_stmt_sem (Seq s s') env mem env'' mem''
+        c_stmt_sem s env mem env' mem' -> 
+        c_stmt_sem s' env' mem' env'' mem'' ->
+        c_stmt_sem (Seq s s') env mem env'' mem''
     | S_Assert env mem e z :
-        env ⊨ e => z -> z <> VInt (FSLZ 0) ->
-        mini_c_stmt_sem (PAssert e) env mem env mem
+        env ⊨ e => z -> z <>  Int.of_z 0 zeroinRange ->
+        c_stmt_sem (PAssert e) env mem env mem
 
-
- where "Ω ',' M '⊨' s '=>' Ω' ',' M'" := (mini_c_stmt_sem s Ω M Ω' M')
+ (* where "Ω ',' M '⊨' s '=>' Ω' ',' M'" := (c_stmt_sem s Ω M Ω' M') *)
     .
 
 (* TODO: mini-fsl *)
